src/NoSync2Stutter.v
@@ -15,705 +15,6 @@ From Fairness Require Export Mod ModSimNoSync ModSimStutter.
 
 Set Implicit Arguments.
 
-(* Section GENORDER. *)
-(*   Context `{M: URA.t}. *)
-
-(*   Variable state_src: Type. *)
-(*   Variable state_tgt: Type. *)
-
-(*   Variable _ident_src: ID. *)
-(*   Definition ident_src := sum_tid _ident_src. *)
-(*   Variable _ident_tgt: ID. *)
-(*   Definition ident_tgt := sum_tid _ident_tgt. *)
-
-(*   Variable wf_src: WF. *)
-(*   Variable wf_tgt: WF. *)
-
-(*   Let srcE := ((@eventE _ident_src +' cE) +' sE state_src). *)
-(*   Let tgtE := ((@eventE _ident_tgt +' cE) +' sE state_tgt). *)
-
-(*   Let shared := *)
-(*     (TIdSet.t * *)
-(*        (@imap ident_src wf_src) * *)
-(*        (@imap ident_tgt wf_tgt) * *)
-(*        state_src * *)
-(*        state_tgt * *)
-(*        URA.car)%type. *)
-
-(*   Let shared_rel: Type := shared -> Prop. *)
-
-(*   Variable I: shared_rel. *)
-
-(*   Let A R0 R1 := (bool * bool * URA.car * (itree srcE R0) * (itree tgtE R1) * shared)%type. *)
-(*   Let wf_ot {R0 R1} := @ord_tree_WF (A R0 R1). *)
-(*   Let wf_stt {R0 R1} := sum_WF (@wf_ot R0 R1) (@wf_ot R0 R1). *)
-
-(*   Variant _geno *)
-(*           (tid: thread_id) *)
-(*           (geno: forall R_src R_tgt (RR: R_src -> R_tgt -> URA.car -> shared_rel), bool -> bool -> URA.car -> ((@wf_stt R_src R_tgt).(T) * itree srcE R_src) -> itree tgtE R_tgt -> shared_rel) *)
-(*           R_src R_tgt (RR: R_src -> R_tgt -> URA.car -> shared_rel) *)
-(*     : *)
-(*     bool -> bool -> URA.car -> ((@wf_stt R_src R_tgt).(T) * itree srcE R_src) -> itree tgtE R_tgt -> shared_rel := *)
-(*   | geno_ret *)
-(*       f_src f_tgt r_ctx o *)
-(*       ths im_src im_tgt st_src st_tgt r_shared *)
-(*       r_src r_tgt *)
-(*       ol or ol0 or0 *)
-(*       (FL: f_src = false -> o = inl ol) *)
-(*       (TR: f_src = true -> o = inr or) *)
-(*       (LTL: wf_ot.(lt) ol0 ol) *)
-(*       (LTR: wf_ot.(lt) or0 or) *)
-(*       (GENO: RR r_src r_tgt r_ctx (ths, im_src, im_tgt, st_src, st_tgt, r_shared)) *)
-(*     : *)
-(*     _geno tid geno RR f_src f_tgt r_ctx (o, Ret r_src) (Ret r_tgt) (ths, im_src, im_tgt, st_src, st_tgt, r_shared) *)
-
-(*   | geno_tauL *)
-(*       f_src f_tgt r_ctx o *)
-(*       ths im_src im_tgt st_src st_tgt r_shared *)
-(*       itr_src itr_tgt *)
-(*       ol or *)
-(*       (FL: f_src = false -> o = inl ol) *)
-(*       (TR: f_src = true -> o = inr or) *)
-(*       o1 (GENO: geno _ _ RR true f_tgt r_ctx (inr o1, itr_src) itr_tgt (ths, im_src, im_tgt, st_src, st_tgt, r_shared)) *)
-(*     : *)
-(*     _geno tid geno RR f_src f_tgt r_ctx (o, Tau itr_src) itr_tgt (ths, im_src, im_tgt, st_src, st_tgt, r_shared) *)
-(*   | geno_chooseL *)
-(*       f_src f_tgt r_ctx o *)
-(*       ths im_src im_tgt st_src st_tgt r_shared *)
-(*       X ktr_src itr_tgt *)
-(*       ol or *)
-(*       (FL: f_src = false -> o = inl ol) *)
-(*       (TR: f_src = true -> o = inr or) *)
-(*       o1 (GENO: exists x, geno _ _ RR true f_tgt r_ctx (inr o1, ktr_src x) itr_tgt (ths, im_src, im_tgt, st_src, st_tgt, r_shared)) *)
-(*     : *)
-(*     _geno tid geno RR f_src f_tgt r_ctx (o, trigger (Choose X) >>= ktr_src) itr_tgt (ths, im_src, im_tgt, st_src, st_tgt, r_shared) *)
-(*   | geno_putL *)
-(*       f_src f_tgt r_ctx o *)
-(*       ths im_src im_tgt st_src st_tgt r_shared *)
-(*       st ktr_src itr_tgt *)
-(*       ol or *)
-(*       (FL: f_src = false -> o = inl ol) *)
-(*       (TR: f_src = true -> o = inr or) *)
-(*       o1 (GENO: geno _ _ RR true f_tgt r_ctx (inr o1, ktr_src tt) itr_tgt (ths, im_src, im_tgt, st, st_tgt, r_shared)) *)
-(*     : *)
-(*     _geno tid geno RR f_src f_tgt r_ctx (o, trigger (Put st) >>= ktr_src) itr_tgt (ths, im_src, im_tgt, st_src, st_tgt, r_shared) *)
-(*   | geno_getL *)
-(*       f_src f_tgt r_ctx o *)
-(*       ths im_src im_tgt st_src st_tgt r_shared *)
-(*       ktr_src itr_tgt *)
-(*       ol or *)
-(*       (FL: f_src = false -> o = inl ol) *)
-(*       (TR: f_src = true -> o = inr or) *)
-(*       o1 (GENO: geno _ _ RR true f_tgt r_ctx (inr o1, ktr_src st_src) itr_tgt (ths, im_src, im_tgt, st_src, st_tgt, r_shared)) *)
-(*     : *)
-(*     _geno tid geno RR f_src f_tgt r_ctx (o, trigger (@Get _) >>= ktr_src) itr_tgt (ths, im_src, im_tgt, st_src, st_tgt, r_shared) *)
-(*   | geno_tidL *)
-(*       f_src f_tgt r_ctx o *)
-(*       ths im_src im_tgt st_src st_tgt r_shared *)
-(*       ktr_src itr_tgt *)
-(*       ol or *)
-(*       (FL: f_src = false -> o = inl ol) *)
-(*       (TR: f_src = true -> o = inr or) *)
-(*       o1 (GENO: geno _ _ RR true f_tgt r_ctx (inr o1, ktr_src tid) itr_tgt (ths, im_src, im_tgt, st_src, st_tgt, r_shared)) *)
-(*     : *)
-(*     _geno tid geno RR f_src f_tgt r_ctx (o, trigger (GetTid) >>= ktr_src) itr_tgt (ths, im_src, im_tgt, st_src, st_tgt, r_shared) *)
-(*   | geno_UB *)
-(*       f_src f_tgt r_ctx o *)
-(*       ths im_src im_tgt st_src st_tgt r_shared *)
-(*       ktr_src itr_tgt *)
-(*       ol or *)
-(*       (FL: f_src = false -> o = inl ol) *)
-(*       (TR: f_src = true -> o = inr or) *)
-(*     : *)
-(*     _geno tid geno RR f_src f_tgt r_ctx (o, trigger (Undefined) >>= ktr_src) itr_tgt (ths, im_src, im_tgt, st_src, st_tgt, r_shared) *)
-(*   | geno_fairL *)
-(*       f_src f_tgt r_ctx o *)
-(*       ths im_src0 im_tgt st_src st_tgt r_shared *)
-(*       f ktr_src itr_tgt *)
-(*       ol or *)
-(*       (FL: f_src = false -> o = inl ol) *)
-(*       (TR: f_src = true -> o = inr or) *)
-(*       o1 (GENO: exists im_src1, *)
-(*              (<<FAIR: fair_update im_src0 im_src1 (sum_fmap_r f)>>) /\ *)
-(*                (<<GENO: geno _ _ RR true f_tgt r_ctx (inr o1, ktr_src tt) itr_tgt (ths, im_src1, im_tgt, st_src, st_tgt, r_shared)>>)) *)
-(*     : *)
-(*     _geno tid geno RR f_src f_tgt r_ctx (o, trigger (Fair f) >>= ktr_src) itr_tgt (ths, im_src0, im_tgt, st_src, st_tgt, r_shared) *)
-
-(*   | geno_tauR *)
-(*       f_src f_tgt r_ctx o *)
-(*       ths im_src im_tgt st_src st_tgt r_shared *)
-(*       itr_src itr_tgt *)
-(*       ol or *)
-(*       (FL: f_src = false -> o = inl ol) *)
-(*       (TR: f_src = true -> o = inr or) *)
-(*       (GENO: geno _ _ RR f_src true r_ctx (o, itr_src) itr_tgt (ths, im_src, im_tgt, st_src, st_tgt, r_shared)) *)
-(*     : *)
-(*     _geno tid geno RR f_src f_tgt r_ctx (o, itr_src) (Tau itr_tgt) (ths, im_src, im_tgt, st_src, st_tgt, r_shared) *)
-(*   | geno_chooseR *)
-(*       f_src f_tgt r_ctx o *)
-(*       ths im_src im_tgt st_src st_tgt r_shared *)
-(*       X itr_src ktr_tgt *)
-(*       ol or *)
-(*       (FL: f_src = false -> o = inl ol) *)
-(*       (TR: f_src = true -> o = inr or) *)
-(*       (GENO: forall x, geno _ _ RR f_src true r_ctx (o, itr_src) (ktr_tgt x) (ths, im_src, im_tgt, st_src, st_tgt, r_shared)) *)
-(*     : *)
-(*     _geno tid geno RR f_src f_tgt r_ctx (o, itr_src) (trigger (Choose X) >>= ktr_tgt) (ths, im_src, im_tgt, st_src, st_tgt, r_shared) *)
-(*   | geno_putR *)
-(*       f_src f_tgt r_ctx o *)
-(*       ths im_src im_tgt st_src st_tgt r_shared *)
-(*       st itr_src ktr_tgt *)
-(*       ol or *)
-(*       (FL: f_src = false -> o = inl ol) *)
-(*       (TR: f_src = true -> o = inr or) *)
-(*       (GENO: geno _ _ RR f_src true r_ctx (o, itr_src) (ktr_tgt tt) (ths, im_src, im_tgt, st_src, st, r_shared)) *)
-(*     : *)
-(*     _geno tid geno RR f_src f_tgt r_ctx (o, itr_src) (trigger (Put st) >>= ktr_tgt) (ths, im_src, im_tgt, st_src, st_tgt, r_shared) *)
-(*   | geno_getR *)
-(*       f_src f_tgt r_ctx o *)
-(*       ths im_src im_tgt st_src st_tgt r_shared *)
-(*       itr_src ktr_tgt *)
-(*       ol or *)
-(*       (FL: f_src = false -> o = inl ol) *)
-(*       (TR: f_src = true -> o = inr or) *)
-(*       (GENO: geno _ _ RR f_src true r_ctx (o, itr_src) (ktr_tgt st_tgt) (ths, im_src, im_tgt, st_src, st_tgt, r_shared)) *)
-(*     : *)
-(*     _geno tid geno RR f_src f_tgt r_ctx (o, itr_src) (trigger (@Get _) >>= ktr_tgt) (ths, im_src, im_tgt, st_src, st_tgt, r_shared) *)
-(*   | geno_tidR *)
-(*       f_src f_tgt r_ctx o *)
-(*       ths im_src im_tgt st_src st_tgt r_shared *)
-(*       itr_src ktr_tgt *)
-(*       ol or *)
-(*       (FL: f_src = false -> o = inl ol) *)
-(*       (TR: f_src = true -> o = inr or) *)
-(*       (GENO: geno _ _ RR f_src true r_ctx (o, itr_src) (ktr_tgt tid) (ths, im_src, im_tgt, st_src, st_tgt, r_shared)) *)
-(*     : *)
-(*     _geno tid geno RR f_src f_tgt r_ctx (o, itr_src) (trigger (GetTid) >>= ktr_tgt) (ths, im_src, im_tgt, st_src, st_tgt, r_shared) *)
-(*   | geno_fairR *)
-(*       f_src f_tgt r_ctx o *)
-(*       ths im_src im_tgt0 st_src st_tgt r_shared *)
-(*       f itr_src ktr_tgt *)
-(*       ol or *)
-(*       (FL: f_src = false -> o = inl ol) *)
-(*       (TR: f_src = true -> o = inr or) *)
-(*       (GENO: forall im_tgt1 *)
-(*                    (FAIR: fair_update im_tgt0 im_tgt1 (sum_fmap_r f)), *)
-(*           (<<GENO: geno _ _ RR f_src true r_ctx (o, itr_src) (ktr_tgt tt) (ths, im_src, im_tgt1, st_src, st_tgt, r_shared)>>)) *)
-(*     : *)
-(*     _geno tid geno RR f_src f_tgt r_ctx (o, itr_src) (trigger (Fair f) >>= ktr_tgt) (ths, im_src, im_tgt0, st_src, st_tgt, r_shared) *)
-
-(*   | geno_observe *)
-(*       f_src f_tgt r_ctx o *)
-(*       ths im_src im_tgt st_src st_tgt r_shared *)
-(*       fn args ktr_src ktr_tgt *)
-(*       ol or *)
-(*       (FL: f_src = false -> o = inl ol) *)
-(*       (TR: f_src = true -> o = inr or) *)
-(*       o1 (GENO: forall ret, *)
-(*              geno _ _ RR true true r_ctx (inr o1, ktr_src ret) (ktr_tgt ret) (ths, im_src, im_tgt, st_src, st_tgt, r_shared)) *)
-(*     : *)
-(*     _geno tid geno RR f_src f_tgt r_ctx (o, trigger (Observe fn args) >>= ktr_src) (trigger (Observe fn args) >>= ktr_tgt) (ths, im_src, im_tgt, st_src, st_tgt, r_shared) *)
-
-(*   | geno_yieldR *)
-(*       f_src f_tgt r_ctx0 o0 *)
-(*       ths0 im_src0 im_tgt0 st_src0 st_tgt0 r_shared0 *)
-(*       r_own r_shared *)
-(*       ktr_src ktr_tgt *)
-(*       ol0 or0 *)
-(*       (FL: f_src = false -> o0 = inl ol0) *)
-(*       (TR: f_src = true -> o0 = inr or0) *)
-(*       (INV: I (ths0, im_src0, im_tgt0, st_src0, st_tgt0, r_shared)) *)
-(*       (VALID: URA.wf (r_shared ⋅ r_own ⋅ r_ctx0)) *)
-(*       (GENOF: (f_src = false) -> *)
-(*               forall ths1 im_src1 im_tgt1 st_src1 st_tgt1 r_shared1 r_ctx1 *)
-(*                 (INV: I (ths1, im_src1, im_tgt1, st_src1, st_tgt1, r_shared1)) *)
-(*                 (VALID: URA.wf (r_shared1 ⋅ r_own ⋅ r_ctx1)) *)
-(*                 im_tgt2 *)
-(*                 (TGT: fair_update im_tgt1 im_tgt2 (sum_fmap_l (tids_fmap tid ths1))), *)
-(*               exists ol1, *)
-(*                 (<<GENO: geno _ _ RR f_src true r_ctx1 (inl ol1, trigger (Yield) >>= ktr_src) (ktr_tgt tt) (ths1, im_src1, im_tgt2, st_src1, st_tgt1, r_shared1)>>) /\ *)
-(*                   (<<STUTTER: wf_ot.(lt) ol1 ol0>>)) *)
-(*       (GENOT: (f_src = true) -> *)
-(*               forall ths1 im_src1 im_tgt1 st_src1 st_tgt1 r_shared1 r_ctx1 *)
-(*                 (INV: I (ths1, im_src1, im_tgt1, st_src1, st_tgt1, r_shared1)) *)
-(*                 (VALID: URA.wf (r_shared1 ⋅ r_own ⋅ r_ctx1)) *)
-(*                 im_tgt2 *)
-(*                 (TGT: fair_update im_tgt1 im_tgt2 (sum_fmap_l (tids_fmap tid ths1))), *)
-(*               exists or1, *)
-(*                 (<<GENO: geno _ _ RR f_src true r_ctx1 (inr or1, trigger (Yield) >>= ktr_src) (ktr_tgt tt) (ths1, im_src1, im_tgt2, st_src1, st_tgt1, r_shared1)>>) /\ *)
-(*                   (<<STUTTER: wf_ot.(lt) or1 or0>>)) *)
-(*     : *)
-(*     _geno tid geno RR f_src f_tgt r_ctx0 (o0, trigger (Yield) >>= ktr_src) (trigger (Yield) >>= ktr_tgt) (ths0, im_src0, im_tgt0, st_src0, st_tgt0, r_shared0) *)
-
-(*   | geno_yieldL *)
-(*       f_src f_tgt r_ctx o0 *)
-(*       ths im_src0 im_tgt st_src st_tgt r_shared *)
-(*       ktr_src itr_tgt *)
-(*       ol0 or0 *)
-(*       (FL: f_src = false -> o0 = inl ol0) *)
-(*       (TR: f_src = true -> o0 = inr or0) *)
-(*       (GENO: exists im_src1 o1, *)
-(*           (<<FAIR: fair_update im_src0 im_src1 (sum_fmap_l (tids_fmap tid ths))>>) /\ *)
-(*             (<<GENO: geno _ _ RR true f_tgt r_ctx (inr o1, ktr_src tt) itr_tgt (ths, im_src1, im_tgt, st_src, st_tgt, r_shared)>>)) *)
-(*     : *)
-(*     _geno tid geno RR f_src f_tgt r_ctx (o0, trigger (Yield) >>= ktr_src) itr_tgt (ths, im_src0, im_tgt, st_src, st_tgt, r_shared) *)
-
-(*   | geno_progress *)
-(*       r_ctx o *)
-(*       ths im_src im_tgt st_src st_tgt r_shared *)
-(*       itr_src itr_tgt *)
-(*       (GENO: ModSimNoSync.lsim I tid RR false false r_ctx itr_src itr_tgt (ths, im_src, im_tgt, st_src, st_tgt, r_shared)) *)
-(*     : *)
-(*     _geno tid geno RR true true r_ctx (inr o, itr_src) itr_tgt (ths, im_src, im_tgt, st_src, st_tgt, r_shared) *)
-(*   . *)
-
-(*   Definition geno (tid: thread_id) *)
-(*              R_src R_tgt (RR: R_src -> R_tgt -> URA.car -> shared_rel): *)
-(*     bool -> bool -> URA.car -> (wf_stt.(T) * itree srcE R_src) -> itree tgtE R_tgt -> shared_rel := *)
-(*     pind9 (_geno tid) top9 R_src R_tgt RR. *)
-
-(*   Lemma geno_mon tid: monotone9 (_geno tid). *)
-(*   Proof. *)
-(*     ii. inv IN; try (econs; eauto; fail). *)
-(*     { des. econs; eauto. } *)
-(*     { des. econs; eauto. } *)
-(*     { econs; eauto. i. eapply LE. eapply GENO. eauto. } *)
-(*     { econs; eauto. *)
-(*       - clear GENOT. i. specialize (GENOF H _ _ _ _ _ _ _ INV0 VALID0 _ TGT). des. esplits; eauto. *)
-(*       - clear GENOF. i. specialize (GENOT H _ _ _ _ _ _ _ INV0 VALID0 _ TGT). des. esplits; eauto. *)
-(*     } *)
-(*     { des. econs; esplits; eauto. } *)
-(*   Qed. *)
-
-(*   Local Hint Constructors _geno: core. *)
-(*   Local Hint Unfold geno: core. *)
-(*   Local Hint Resolve geno_mon: paco. *)
-
-(*   (* Properties *) *)
-(*   Lemma geno_sfalse_oright *)
-(*         tid R0 R1 (RR: R0 -> R1 -> URA.car -> shared_rel) *)
-(*         pt r_ctx src tgt shr o *)
-(*     : *)
-(*     ~ (geno tid RR false pt r_ctx (inr o, src) tgt shr). *)
-(*   Proof. *)
-(*     intros GENO. *)
-(*     match goal with | GENO: geno _ _ ?_ps _ _ ?_osrc _ _ |- _ => remember _ps as ps; remember _osrc as osrc end. *)
-(*     move GENO before tid. revert_until GENO. *)
-(*     pattern R0, R1, RR, ps, pt, r_ctx, osrc, tgt, shr. *)
-(*     revert R0 R1 RR ps pt r_ctx osrc tgt shr GENO. apply pind9_acc. *)
-(*     intros rr DEC IH. clear DEC. intros R0 R1 RR ps pt r_ctx osrc tgt shr GENO. *)
-(*     i; clarify. *)
-(*     eapply pind9_unfold in GENO; eauto with paco. *)
-(*     inv GENO; try (hexploit FL; ss; fail). *)
-(*   Qed. *)
-
-(*   Lemma geno_strue_oleft *)
-(*         tid R0 R1 (RR: R0 -> R1 -> URA.car -> shared_rel) *)
-(*         pt r_ctx src tgt shr o *)
-(*     : *)
-(*     ~ (geno tid RR true pt r_ctx (inl o, src) tgt shr). *)
-(*   Proof. *)
-(*     intros GENO. *)
-(*     match goal with | GENO: geno _ _ ?_ps _ _ ?_osrc _ _ |- _ => remember _ps as ps; remember _osrc as osrc end. *)
-(*     move GENO before tid. revert_until GENO. *)
-(*     pattern R0, R1, RR, ps, pt, r_ctx, osrc, tgt, shr. *)
-(*     revert R0 R1 RR ps pt r_ctx osrc tgt shr GENO. apply pind9_acc. *)
-(*     intros rr DEC IH. clear DEC. intros R0 R1 RR ps pt r_ctx osrc tgt shr GENO. *)
-(*     i; clarify. *)
-(*     eapply pind9_unfold in GENO; eauto with paco. *)
-(*     inv GENO; try (hexploit TR; ss; fail). *)
-(*   Qed. *)
-
-(*   Lemma geno_ord_weak_left *)
-(*         tid R0 R1 (LRR: R0 -> R1 -> URA.car -> shared_rel) *)
-(*         ps pt r_ctx src tgt (shr: shared) o0 o1 *)
-(*         (LT: wf_ot.(lt) o0 o1) *)
-(*         (GENO: geno tid LRR ps pt r_ctx (inl o0, src) tgt shr) *)
-(*     : *)
-(*     geno tid LRR ps pt r_ctx (inl o1, src) tgt shr. *)
-(*   Proof. *)
-(*     remember (inl o0, src) as osrc. *)
-(*     move GENO before tid. revert_until GENO. *)
-(*     pattern R0, R1, LRR, ps, pt, r_ctx, osrc, tgt, shr. *)
-(*     revert R0 R1 LRR ps pt r_ctx osrc tgt shr GENO. apply pind9_acc. *)
-(*     intros rr DEC IH. clear DEC. intros R0 R1 LRR ps pt r_ctx osrc tgt shr GENO. *)
-(*     i; clarify. *)
-(*     eapply pind9_unfold in GENO; eauto with paco. *)
-(*     inv GENO. *)
-
-(*     { eapply pind9_fold. econs 1; eauto. i. apply TR in H; ss. } *)
-(*     { eapply pind9_fold. econs 2; eauto. i. apply TR in H; ss. *)
-(*       eapply upind9_mon; eauto. ss. *)
-(*       Unshelve. exact o2. *)
-(*     } *)
-(*     { eapply pind9_fold. econs 3; eauto. i. apply TR in H; ss. *)
-(*       des. exists x. *)
-(*       eapply upind9_mon; eauto. ss. *)
-(*       Unshelve. exact o2. *)
-(*     } *)
-(*     { eapply pind9_fold. econs 4; eauto. i. apply TR in H; ss. *)
-(*       eapply upind9_mon; eauto. ss. *)
-(*       Unshelve. exact o2. *)
-(*     } *)
-(*     { eapply pind9_fold. econs 5; eauto. i. apply TR in H; ss. *)
-(*       eapply upind9_mon; eauto. ss. *)
-(*       Unshelve. exact o2. *)
-(*     } *)
-(*     { eapply pind9_fold. econs 6; eauto. i. apply TR in H; ss. *)
-(*       eapply upind9_mon; eauto. ss. *)
-(*       Unshelve. exact o2. *)
-(*     } *)
-(*     { eapply pind9_fold. econs 7; eauto. i. apply TR in H; ss. *)
-(*       Unshelve. exact o0. *)
-(*     } *)
-(*     { eapply pind9_fold. econs 8; eauto. i. apply TR in H; ss. *)
-(*       des. esplits; eauto. *)
-(*       eapply upind9_mon; eauto. ss. *)
-(*       Unshelve. exact o2. *)
-(*     } *)
-
-(*     { eapply pind9_fold. econs 9; eauto. i. apply TR in H; ss. *)
-(*       split; ss. destruct GENO0 as [GENO IND]. eapply IH in IND; eauto. *)
-(*       Unshelve. exact o1. *)
-(*     } *)
-(*     { eapply pind9_fold. econs 10; eauto. i. apply TR in H; ss. *)
-(*       i. specialize (GENO0 x). *)
-(*       split; ss. destruct GENO0 as [GENO IND]. eapply IH in IND; eauto. *)
-(*       Unshelve. exact o1. *)
-(*     } *)
-(*     { eapply pind9_fold. econs 11; eauto. i. apply TR in H; ss. *)
-(*       split; ss. destruct GENO0 as [GENO IND]. eapply IH in IND; eauto. *)
-(*       Unshelve. exact o1. *)
-(*     } *)
-(*     { eapply pind9_fold. econs 12; eauto. i. apply TR in H; ss. *)
-(*       split; ss. destruct GENO0 as [GENO IND]. eapply IH in IND; eauto. *)
-(*       Unshelve. exact o1. *)
-(*     } *)
-(*     { eapply pind9_fold. econs 13; eauto. i. apply TR in H; ss. *)
-(*       split; ss. destruct GENO0 as [GENO IND]. eapply IH in IND; eauto. *)
-(*       Unshelve. exact o1. *)
-(*     } *)
-(*     { eapply pind9_fold. econs 14; eauto. i. apply TR in H; ss. *)
-(*       i. specialize (GENO0 _ FAIR). *)
-(*       split; ss. destruct GENO0 as [GENO IND]. eapply IH in IND; eauto. *)
-(*       Unshelve. exact o1. *)
-(*     } *)
-(*     { eapply pind9_fold. econs 15; eauto. i. apply TR in H; ss. *)
-(*       i. specialize (GENO0 ret). *)
-(*       eapply upind9_mon; eauto. ss. *)
-(*       Unshelve. exact o2. *)
-(*     } *)
-
-(*     { eapply pind9_fold. econs 16; eauto. i. apply TR in H; ss. *)
-(*       - i. clear GENOT. specialize (GENOF H _ _ _ _ _ _ _ INV0 VALID0 _ TGT). *)
-(*         des. esplits; eauto. *)
-(*         split; ss. destruct GENO as [GENO IND]. eapply IH in IND; eauto. *)
-(*         apply FL in H. clarify. *)
-(*         Unshelve. exact o1. *)
-(*       - i. clear GENOF. apply TR in H; ss. *)
-(*     } *)
-
-(*     { eapply pind9_fold. econs 17; eauto. i. apply TR in H; ss. *)
-(*       des. esplits; eauto. destruct GENO as [GENO IND]. *)
-(*       eapply upind9_mon; eauto. ss. *)
-(*       Unshelve. exact o1. *)
-(*     } *)
-
-(*   Qed. *)
-
-(*   Lemma geno_ord_weak_right *)
-(*         tid R0 R1 (LRR: R0 -> R1 -> URA.car -> shared_rel) *)
-(*         ps pt r_ctx src tgt (shr: shared) o0 o1 *)
-(*         (LT: wf_ot.(lt) o0 o1) *)
-(*         (GENO: geno tid LRR ps pt r_ctx (inr o0, src) tgt shr) *)
-(*     : *)
-(*     geno tid LRR ps pt r_ctx (inr o1, src) tgt shr. *)
-(*   Proof. *)
-(*     remember (inr o0, src) as osrc. *)
-(*     move GENO before tid. revert_until GENO. *)
-(*     pattern R0, R1, LRR, ps, pt, r_ctx, osrc, tgt, shr. *)
-(*     revert R0 R1 LRR ps pt r_ctx osrc tgt shr GENO. apply pind9_acc. *)
-(*     intros rr DEC IH. clear DEC. intros R0 R1 LRR ps pt r_ctx osrc tgt shr GENO. *)
-(*     i; clarify. *)
-(*     eapply pind9_unfold in GENO; eauto with paco. *)
-(*     inv GENO. *)
-
-(*     { eapply pind9_fold. econs 1; eauto. i. apply FL in H; ss. } *)
-(*     { eapply pind9_fold. econs 2; eauto. i. apply FL in H; ss. *)
-(*       eapply upind9_mon; eauto. ss. *)
-(*       Unshelve. exact o2. *)
-(*     } *)
-(*     { eapply pind9_fold. econs 3; eauto. i. apply FL in H; ss. *)
-(*       des. exists x. *)
-(*       eapply upind9_mon; eauto. ss. *)
-(*       Unshelve. exact o2. *)
-(*     } *)
-(*     { eapply pind9_fold. econs 4; eauto. i. apply FL in H; ss. *)
-(*       eapply upind9_mon; eauto. ss. *)
-(*       Unshelve. exact o2. *)
-(*     } *)
-(*     { eapply pind9_fold. econs 5; eauto. i. apply FL in H; ss. *)
-(*       eapply upind9_mon; eauto. ss. *)
-(*       Unshelve. exact o2. *)
-(*     } *)
-(*     { eapply pind9_fold. econs 6; eauto. i. apply FL in H; ss. *)
-(*       eapply upind9_mon; eauto. ss. *)
-(*       Unshelve. exact o2. *)
-(*     } *)
-(*     { eapply pind9_fold. econs 7; eauto. i. apply FL in H; ss. *)
-(*       Unshelve. exact o0. *)
-(*     } *)
-(*     { eapply pind9_fold. econs 8; eauto. i. apply FL in H; ss. *)
-(*       des. esplits; eauto. *)
-(*       eapply upind9_mon; eauto. ss. *)
-(*       Unshelve. exact o2. *)
-(*     } *)
-
-(*     { eapply pind9_fold. econs 9; eauto. i. apply FL in H; ss. *)
-(*       split; ss. destruct GENO0 as [GENO IND]. eapply IH in IND; eauto. *)
-(*       Unshelve. exact o1. *)
-(*     } *)
-(*     { eapply pind9_fold. econs 10; eauto. i. apply FL in H; ss. *)
-(*       i. specialize (GENO0 x). *)
-(*       split; ss. destruct GENO0 as [GENO IND]. eapply IH in IND; eauto. *)
-(*       Unshelve. exact o1. *)
-(*     } *)
-(*     { eapply pind9_fold. econs 11; eauto. i. apply FL in H; ss. *)
-(*       split; ss. destruct GENO0 as [GENO IND]. eapply IH in IND; eauto. *)
-(*       Unshelve. exact o1. *)
-(*     } *)
-(*     { eapply pind9_fold. econs 12; eauto. i. apply FL in H; ss. *)
-(*       split; ss. destruct GENO0 as [GENO IND]. eapply IH in IND; eauto. *)
-(*       Unshelve. exact o1. *)
-(*     } *)
-(*     { eapply pind9_fold. econs 13; eauto. i. apply FL in H; ss. *)
-(*       split; ss. destruct GENO0 as [GENO IND]. eapply IH in IND; eauto. *)
-(*       Unshelve. exact o1. *)
-(*     } *)
-(*     { eapply pind9_fold. econs 14; eauto. i. apply FL in H; ss. *)
-(*       i. specialize (GENO0 _ FAIR). *)
-(*       split; ss. destruct GENO0 as [GENO IND]. eapply IH in IND; eauto. *)
-(*       Unshelve. exact o1. *)
-(*     } *)
-(*     { eapply pind9_fold. econs 15; eauto. i. apply FL in H; ss. *)
-(*       i. specialize (GENO0 ret). *)
-(*       eapply upind9_mon; eauto. ss. *)
-(*       Unshelve. exact o2. *)
-(*     } *)
-
-(*     { eapply pind9_fold. econs 16; eauto. i. apply FL in H; ss. *)
-(*       - i. clear GENOT. apply FL in H; ss. *)
-(*       - i. clear GENOF. specialize (GENOT H _ _ _ _ _ _ _ INV0 VALID0 _ TGT). *)
-(*         des. esplits; eauto. *)
-(*         split; ss. destruct GENO as [GENO IND]. eapply IH in IND; eauto. *)
-(*         apply TR in H. clarify. *)
-(*         Unshelve. exact o1. *)
-(*     } *)
-
-(*     { eapply pind9_fold. econs 17; eauto. i. apply FL in H; ss. *)
-(*       des. esplits; eauto. destruct GENO as [GENO IND]. *)
-(*       eapply upind9_mon; eauto. ss. *)
-(*       Unshelve. exact o1. *)
-(*     } *)
-
-(*     { eapply pind9_fold. econs 18; eauto. } *)
-
-(*   Qed. *)
-
-(*   Lemma nosync_geno *)
-(*         tid R0 R1 (RR: R0 -> R1 -> URA.car -> shared_rel) *)
-(*         ps pt r_ctx src tgt shr *)
-(*         (LSIM: ModSimNoSync.lsim I tid RR ps pt r_ctx src tgt shr) *)
-(*     : *)
-(*     exists o, geno tid RR ps pt r_ctx (o, src) tgt shr. *)
-(*   Proof. *)
-(*     punfold LSIM. *)
-(*     pattern R0, R1, RR, ps, pt, r_ctx, src, tgt, shr. *)
-(*     revert R0 R1 RR ps pt r_ctx src tgt shr LSIM. apply pind9_acc. *)
-(*     intros rr DEC IH. clear DEC. intros R0 R1 RR ps pt r_ctx src tgt shr LSIM. *)
-(*     eapply pind9_unfold in LSIM; eauto with paco. *)
-(*     (* specialize (one R0 R1). specialize (@fzero R0 R1). *) *)
-(*     set (fzero:= fun _: (A R0 R1) => @ord_tree_base (A R0 R1)). set (one:= ord_tree_cons fzero). *)
-(*     inv LSIM. *)
-
-(*     { exists (if ps then (inr one) else (inl one)). *)
-(*       eapply pind9_fold. econs 1; eauto. des_ifs. des_ifs. *)
-(*       1,2: instantiate (1:=fzero (ps, pt, r_ctx, Ret r_src, Ret r_tgt, (ths, im_src, im_tgt, st_src, st_tgt, r_shared))); ss. *)
-(*     } *)
-
-(*     { exists (if ps then (inr one) else (inl one)). *)
-(*       destruct LSIM0 as [LSIM IND]. eapply IH in IND. des. *)
-(*       destruct o. apply geno_strue_oleft in IND; ss. *)
-(*       eapply pind9_fold. econs 2; eauto. 1,2: des_ifs. *)
-(*       split; ss. eauto. *)
-(*     } *)
-(*     { exists (if ps then (inr one) else (inl one)). *)
-(*       des. destruct LSIM0 as [LSIM IND]. eapply IH in IND. des. *)
-(*       destruct o. apply geno_strue_oleft in IND; ss. *)
-(*       eapply pind9_fold. econs 3; eauto. 1,2: des_ifs. *)
-(*       eexists; split; ss. eauto. *)
-(*     } *)
-(*     { exists (if ps then (inr one) else (inl one)). *)
-(*       destruct LSIM0 as [LSIM IND]. eapply IH in IND. des. *)
-(*       destruct o. apply geno_strue_oleft in IND; ss. *)
-(*       eapply pind9_fold. econs 4; eauto. 1,2: des_ifs. *)
-(*       split; ss. eauto. *)
-(*     } *)
-(*     { exists (if ps then (inr one) else (inl one)). *)
-(*       destruct LSIM0 as [LSIM IND]. eapply IH in IND. des. *)
-(*       destruct o. apply geno_strue_oleft in IND; ss. *)
-(*       eapply pind9_fold. econs 5; eauto. 1,2: des_ifs. *)
-(*       split; ss. eauto. *)
-(*     } *)
-(*     { exists (if ps then (inr one) else (inl one)). *)
-(*       destruct LSIM0 as [LSIM IND]. eapply IH in IND. des. *)
-(*       destruct o. apply geno_strue_oleft in IND; ss. *)
-(*       eapply pind9_fold. econs 6; eauto. 1,2: des_ifs. *)
-(*       split; ss. eauto. *)
-(*     } *)
-(*     { exists (if ps then (inr one) else (inl one)). *)
-(*       eapply pind9_fold. econs 7; eauto. 1,2: des_ifs. *)
-(*     } *)
-(*     { exists (if ps then (inr one) else (inl one)). *)
-(*       des. destruct LSIM as [LSIM IND]. eapply IH in IND. des. *)
-(*       destruct o. apply geno_strue_oleft in IND; ss. *)
-(*       eapply pind9_fold. econs 8; eauto. 1,2: des_ifs. *)
-(*       esplits; eauto. split; ss. eauto. *)
-(*     } *)
-
-(*     { destruct LSIM0 as [LSIM IND]. eapply IH in IND. des. exists o. *)
-(*       destruct ps; destruct o. *)
-(*       1:{ apply geno_strue_oleft in IND; ss. } *)
-(*       3:{ apply geno_sfalse_oright in IND; ss. } *)
-(*       - eapply pind9_fold. econs 9; eauto. ss. split; ss; auto. *)
-(*       - eapply pind9_fold. econs 9; eauto. ss. split; ss; auto. *)
-(*         Unshelve. all: exact t. *)
-(*     } *)
-
-(*     { hexploit ord_tree_join. *)
-(*       { instantiate (2:=A R0 R1). *)
-(*         instantiate (2:= fun '(ps, pt, rs, src, tgt, shr) => @rr R0 R1 RR ps pt rs src tgt shr). *)
-(*         i. ss. des_ifs. eapply IH in SAT. *)
-(*         instantiate (1:= fun '(ps, pt, rs, src, tgt, shr) o => *)
-(*                            geno tid RR ps pt rs (if ps then (inr o) else (inl o), src) tgt shr). *)
-(*         des. destruct b; destruct o. *)
-(*         1:{ apply geno_strue_oleft in SAT; ss. } *)
-(*         3:{ apply geno_sfalse_oright in SAT; ss. } *)
-(*         all: eauto. *)
-(*       } *)
-(*       intro JOIN. des. exists (if ps then (inr o1) else (inl o1)). *)
-(*       eapply pind9_fold. econs 10. 1,2: des_ifs. *)
-(*       i. specialize (LSIM0 x). destruct LSIM0 as [LSIM IND]. *)
-(*       specialize (JOIN (ps, true, r_ctx, src, (ktr_tgt x), (ths, im_src, im_tgt, st_src, st_tgt, r_shared))). *)
-(*       destruct JOIN; auto. des. split; ss. des_ifs. *)
-(*       eapply geno_ord_weak_right; eauto. *)
-(*       eapply geno_ord_weak_left; eauto. *)
-(*     } *)
-
-(*     { destruct LSIM0 as [LSIM IND]. eapply IH in IND. des. exists o. *)
-(*       destruct ps; destruct o. *)
-(*       1:{ apply geno_strue_oleft in IND; ss. } *)
-(*       3:{ apply geno_sfalse_oright in IND; ss. } *)
-(*       - eapply pind9_fold. econs 11; eauto. ss. split; ss; auto. *)
-(*       - eapply pind9_fold. econs 11; eauto. ss. split; ss; auto. *)
-(*         Unshelve. all: exact t. *)
-(*     } *)
-(*     { destruct LSIM0 as [LSIM IND]. eapply IH in IND. des. exists o. *)
-(*       destruct ps; destruct o. *)
-(*       1:{ apply geno_strue_oleft in IND; ss. } *)
-(*       3:{ apply geno_sfalse_oright in IND; ss. } *)
-(*       - eapply pind9_fold. econs 12; eauto. ss. split; ss; auto. *)
-(*       - eapply pind9_fold. econs 12; eauto. ss. split; ss; auto. *)
-(*         Unshelve. all: exact t. *)
-(*     } *)
-(*     { destruct LSIM0 as [LSIM IND]. eapply IH in IND. des. exists o. *)
-(*       destruct ps; destruct o. *)
-(*       1:{ apply geno_strue_oleft in IND; ss. } *)
-(*       3:{ apply geno_sfalse_oright in IND; ss. } *)
-(*       - eapply pind9_fold. econs 13; eauto. ss. split; ss; auto. *)
-(*       - eapply pind9_fold. econs 13; eauto. ss. split; ss; auto. *)
-(*         Unshelve. all: exact t. *)
-(*     } *)
-
-(*     { hexploit ord_tree_join. *)
-(*       { instantiate (2:=A R0 R1). *)
-(*         instantiate (2:= fun '(ps, pt, rs, src, tgt, shr) => @rr R0 R1 RR ps pt rs src tgt shr). *)
-(*         i. ss. des_ifs. eapply IH in SAT. *)
-(*         instantiate (1:= fun '(ps, pt, rs, src, tgt, shr) o => *)
-(*                            geno tid RR ps pt rs (if ps then (inr o) else (inl o), src) tgt shr). *)
-(*         des. destruct b; destruct o. *)
-(*         1:{ apply geno_strue_oleft in SAT; ss. } *)
-(*         3:{ apply geno_sfalse_oright in SAT; ss. } *)
-(*         all: eauto. *)
-(*       } *)
-(*       intro JOIN. des. exists (if ps then (inr o1) else (inl o1)). *)
-(*       eapply pind9_fold. econs 14. 1,2: des_ifs. *)
-(*       i. specialize (LSIM0 _ FAIR). destruct LSIM0 as [LSIM IND]. *)
-(*       specialize (JOIN (ps, true, r_ctx, src, (ktr_tgt ()), (ths, im_src, im_tgt1, st_src, st_tgt, r_shared))). *)
-(*       destruct JOIN; auto. des. split; ss. des_ifs. *)
-(*       eapply geno_ord_weak_right; eauto. *)
-(*       eapply geno_ord_weak_left; eauto. *)
-(*     } *)
-
-(*     { hexploit ord_tree_join. *)
-(*       { instantiate (2:=A R0 R1). *)
-(*         instantiate (2:= fun '(ps, pt, rs, src, tgt, shr) => @rr R0 R1 RR ps pt rs src tgt shr). *)
-(*         i. ss. des_ifs. eapply IH in SAT. *)
-(*         instantiate (1:= fun '(ps, pt, rs, src, tgt, shr) o => *)
-(*                            geno tid RR ps pt rs (if ps then (inr o) else (inl o), src) tgt shr). *)
-(*         des. destruct b; destruct o. *)
-(*         1:{ apply geno_strue_oleft in SAT; ss. } *)
-(*         3:{ apply geno_sfalse_oright in SAT; ss. } *)
-(*         all: eauto. *)
-(*       } *)
-(*       intro JOIN. des. exists (if ps then (inr o1) else (inl o1)). *)
-(*       eapply pind9_fold. econs 15. 1,2: des_ifs. *)
-(*       i. specialize (LSIM0 ret). destruct LSIM0 as [LSIM IND]. *)
-(*       specialize (JOIN (true, true, r_ctx, ktr_src ret, ktr_tgt ret, (ths, im_src, im_tgt, st_src, st_tgt, r_shared))). *)
-(*       destruct JOIN; auto. des. split; ss. *)
-(*       eapply geno_ord_weak_right; eauto. *)
-(*     } *)
-
-(*     { hexploit ord_tree_join. *)
-(*       { instantiate (2:=A R0 R1). *)
-(*         instantiate (2:= fun '(ps, pt, rs, src, tgt, shr) => @rr R0 R1 RR ps pt rs src tgt shr). *)
-(*         i. ss. des_ifs. eapply IH in SAT. *)
-(*         instantiate (1:= fun '(ps, pt, rs, src, tgt, shr) o => *)
-(*                            geno tid RR ps pt rs (if ps then (inr o) else (inl o), src) tgt shr). *)
-(*         des. destruct b; destruct o. *)
-(*         1:{ apply geno_strue_oleft in SAT; ss. } *)
-(*         3:{ apply geno_sfalse_oright in SAT; ss. } *)
-(*         all: eauto. *)
-(*       } *)
-(*       intro JOIN. des. exists (if ps then (inr o1) else (inl o1)). *)
-(*       eapply pind9_fold. econs 16. 1,2: des_ifs. *)
-(*       1,2: eauto. *)
-(*       - i. specialize (LSIM0 _ _ _ _ _ _ _ INV0 VALID0 _ TGT). destruct LSIM0 as [LSIM IND]. *)
-(*         specialize (JOIN (ps, true, r_ctx1, (x <- trigger Yield;; ktr_src x), ktr_tgt (), (ths1, im_src1, im_tgt2, st_src1, st_tgt1, r_shared1))). *)
-(*         destruct JOIN; auto. des. clarify. esplits; eauto. split; ss. *)
-(*       - i. specialize (LSIM0 _ _ _ _ _ _ _ INV0 VALID0 _ TGT). destruct LSIM0 as [LSIM IND]. *)
-(*         specialize (JOIN (ps, true, r_ctx1, (x <- trigger Yield;; ktr_src x), ktr_tgt (), (ths1, im_src1, im_tgt2, st_src1, st_tgt1, r_shared1))). *)
-(*         destruct JOIN; auto. des. clarify. esplits; eauto. split; ss. *)
-(*     } *)
-
-(*     { des. destruct LSIM as [LSIM IND]. eapply IH in IND. des. *)
-(*       destruct o. apply geno_strue_oleft in IND; ss. *)
-(*       exists (if ps then (inr one) else (inl one)). *)
-(*       eapply pind9_fold. econs 17; eauto. 1,2: des_ifs. esplits; eauto. *)
-(*       split; ss. eauto. *)
-(*     } *)
-
-(*     { exists (inr (@ord_tree_base _)). eapply pind9_fold. econs 18. pclearbot. auto. } *)
-
-(*   Qed. *)
-
-(*   (*TODO: reduction lemmas*) *)
-
-(* End GENORDER. *)
-(* #[export] Hint Constructors _geno: core. *)
-(* #[export] Hint Unfold geno: core. *)
-(* #[export] Hint Resolve geno_mon: paco. *)
-
 Section GENORDER.
   Context `{M: URA.t}.
 
@@ -747,9 +48,9 @@ Section GENORDER.
   Let wf_stt {R0 R1} := @ord_tree_WF (A R0 R1).
 
   Variant _geno
-          (tid: thread_id)
-          (geno: forall R_src R_tgt (RR: R_src -> R_tgt -> URA.car -> shared_rel), bool -> bool -> URA.car -> ((@wf_stt R_src R_tgt).(T) * itree srcE R_src) -> itree tgtE R_tgt -> shared_rel)
-          R_src R_tgt (RR: R_src -> R_tgt -> URA.car -> shared_rel)
+          (tid: thread_id) R_src R_tgt
+          (geno: forall (RR: R_src -> R_tgt -> URA.car -> shared_rel), bool -> bool -> URA.car -> ((@wf_stt R_src R_tgt).(T) * itree srcE R_src) -> itree tgtE R_tgt -> shared_rel)
+          (RR: R_src -> R_tgt -> URA.car -> shared_rel)
     :
     bool -> bool -> URA.car -> ((@wf_stt R_src R_tgt).(T) * itree srcE R_src) -> itree tgtE R_tgt -> shared_rel :=
   | geno_ret
@@ -765,35 +66,35 @@ Section GENORDER.
       f_src f_tgt r_ctx o
       ths im_src im_tgt st_src st_tgt r_shared
       itr_src itr_tgt
-      (GENO: geno _ _ RR true f_tgt r_ctx (o, itr_src) itr_tgt (ths, im_src, im_tgt, st_src, st_tgt, r_shared))
+      (GENO: geno RR true f_tgt r_ctx (o, itr_src) itr_tgt (ths, im_src, im_tgt, st_src, st_tgt, r_shared))
     :
     _geno tid geno RR f_src f_tgt r_ctx (o, Tau itr_src) itr_tgt (ths, im_src, im_tgt, st_src, st_tgt, r_shared)
   | geno_chooseL
       f_src f_tgt r_ctx o
       ths im_src im_tgt st_src st_tgt r_shared
       X ktr_src itr_tgt
-      (GENO: exists x, geno _ _ RR true f_tgt r_ctx (o, ktr_src x) itr_tgt (ths, im_src, im_tgt, st_src, st_tgt, r_shared))
+      (GENO: exists x, geno RR true f_tgt r_ctx (o, ktr_src x) itr_tgt (ths, im_src, im_tgt, st_src, st_tgt, r_shared))
     :
     _geno tid geno RR f_src f_tgt r_ctx (o, trigger (Choose X) >>= ktr_src) itr_tgt (ths, im_src, im_tgt, st_src, st_tgt, r_shared)
   | geno_putL
       f_src f_tgt r_ctx o
       ths im_src im_tgt st_src st_tgt r_shared
       st ktr_src itr_tgt
-      (GENO: geno _ _ RR true f_tgt r_ctx (o, ktr_src tt) itr_tgt (ths, im_src, im_tgt, st, st_tgt, r_shared))
+      (GENO: geno RR true f_tgt r_ctx (o, ktr_src tt) itr_tgt (ths, im_src, im_tgt, st, st_tgt, r_shared))
     :
     _geno tid geno RR f_src f_tgt r_ctx (o, trigger (Put st) >>= ktr_src) itr_tgt (ths, im_src, im_tgt, st_src, st_tgt, r_shared)
   | geno_getL
       f_src f_tgt r_ctx o
       ths im_src im_tgt st_src st_tgt r_shared
       ktr_src itr_tgt
-      (GENO: geno _ _ RR true f_tgt r_ctx (o, ktr_src st_src) itr_tgt (ths, im_src, im_tgt, st_src, st_tgt, r_shared))
+      (GENO: geno RR true f_tgt r_ctx (o, ktr_src st_src) itr_tgt (ths, im_src, im_tgt, st_src, st_tgt, r_shared))
     :
     _geno tid geno RR f_src f_tgt r_ctx (o, trigger (@Get _) >>= ktr_src) itr_tgt (ths, im_src, im_tgt, st_src, st_tgt, r_shared)
   | geno_tidL
       f_src f_tgt r_ctx o
       ths im_src im_tgt st_src st_tgt r_shared
       ktr_src itr_tgt
-      (GENO: geno _ _ RR true f_tgt r_ctx (o, ktr_src tid) itr_tgt (ths, im_src, im_tgt, st_src, st_tgt, r_shared))
+      (GENO: geno RR true f_tgt r_ctx (o, ktr_src tid) itr_tgt (ths, im_src, im_tgt, st_src, st_tgt, r_shared))
     :
     _geno tid geno RR f_src f_tgt r_ctx (o, trigger (GetTid) >>= ktr_src) itr_tgt (ths, im_src, im_tgt, st_src, st_tgt, r_shared)
   | geno_UB
@@ -808,7 +109,7 @@ Section GENORDER.
       f ktr_src itr_tgt
       (GENO: exists im_src1,
              (<<FAIR: fair_update im_src0 im_src1 (sum_fmap_r f)>>) /\
-               (<<GENO: geno _ _ RR true f_tgt r_ctx (o, ktr_src tt) itr_tgt (ths, im_src1, im_tgt, st_src, st_tgt, r_shared)>>))
+               (<<GENO: geno RR true f_tgt r_ctx (o, ktr_src tt) itr_tgt (ths, im_src1, im_tgt, st_src, st_tgt, r_shared)>>))
     :
     _geno tid geno RR f_src f_tgt r_ctx (o, trigger (Fair f) >>= ktr_src) itr_tgt (ths, im_src0, im_tgt, st_src, st_tgt, r_shared)
 
@@ -816,35 +117,35 @@ Section GENORDER.
       f_src f_tgt r_ctx o
       ths im_src im_tgt st_src st_tgt r_shared
       itr_src itr_tgt
-      (GENO: geno _ _ RR f_src true r_ctx (o, itr_src) itr_tgt (ths, im_src, im_tgt, st_src, st_tgt, r_shared))
+      (GENO: geno RR f_src true r_ctx (o, itr_src) itr_tgt (ths, im_src, im_tgt, st_src, st_tgt, r_shared))
     :
     _geno tid geno RR f_src f_tgt r_ctx (o, itr_src) (Tau itr_tgt) (ths, im_src, im_tgt, st_src, st_tgt, r_shared)
   | geno_chooseR
       f_src f_tgt r_ctx o
       ths im_src im_tgt st_src st_tgt r_shared
       X itr_src ktr_tgt
-      (GENO: forall x, geno _ _ RR f_src true r_ctx (o, itr_src) (ktr_tgt x) (ths, im_src, im_tgt, st_src, st_tgt, r_shared))
+      (GENO: forall x, geno RR f_src true r_ctx (o, itr_src) (ktr_tgt x) (ths, im_src, im_tgt, st_src, st_tgt, r_shared))
     :
     _geno tid geno RR f_src f_tgt r_ctx (o, itr_src) (trigger (Choose X) >>= ktr_tgt) (ths, im_src, im_tgt, st_src, st_tgt, r_shared)
   | geno_putR
       f_src f_tgt r_ctx o
       ths im_src im_tgt st_src st_tgt r_shared
       st itr_src ktr_tgt
-      (GENO: geno _ _ RR f_src true r_ctx (o, itr_src) (ktr_tgt tt) (ths, im_src, im_tgt, st_src, st, r_shared))
+      (GENO: geno RR f_src true r_ctx (o, itr_src) (ktr_tgt tt) (ths, im_src, im_tgt, st_src, st, r_shared))
     :
     _geno tid geno RR f_src f_tgt r_ctx (o, itr_src) (trigger (Put st) >>= ktr_tgt) (ths, im_src, im_tgt, st_src, st_tgt, r_shared)
   | geno_getR
       f_src f_tgt r_ctx o
       ths im_src im_tgt st_src st_tgt r_shared
       itr_src ktr_tgt
-      (GENO: geno _ _ RR f_src true r_ctx (o, itr_src) (ktr_tgt st_tgt) (ths, im_src, im_tgt, st_src, st_tgt, r_shared))
+      (GENO: geno RR f_src true r_ctx (o, itr_src) (ktr_tgt st_tgt) (ths, im_src, im_tgt, st_src, st_tgt, r_shared))
     :
     _geno tid geno RR f_src f_tgt r_ctx (o, itr_src) (trigger (@Get _) >>= ktr_tgt) (ths, im_src, im_tgt, st_src, st_tgt, r_shared)
   | geno_tidR
       f_src f_tgt r_ctx o
       ths im_src im_tgt st_src st_tgt r_shared
       itr_src ktr_tgt
-      (GENO: geno _ _ RR f_src true r_ctx (o, itr_src) (ktr_tgt tid) (ths, im_src, im_tgt, st_src, st_tgt, r_shared))
+      (GENO: geno RR f_src true r_ctx (o, itr_src) (ktr_tgt tid) (ths, im_src, im_tgt, st_src, st_tgt, r_shared))
     :
     _geno tid geno RR f_src f_tgt r_ctx (o, itr_src) (trigger (GetTid) >>= ktr_tgt) (ths, im_src, im_tgt, st_src, st_tgt, r_shared)
   | geno_fairR
@@ -853,7 +154,7 @@ Section GENORDER.
       f itr_src ktr_tgt
       (GENO: forall im_tgt1
                    (FAIR: fair_update im_tgt0 im_tgt1 (sum_fmap_r f)),
-          (<<GENO: geno _ _ RR f_src true r_ctx (o, itr_src) (ktr_tgt tt) (ths, im_src, im_tgt1, st_src, st_tgt, r_shared)>>))
+          (<<GENO: geno RR f_src true r_ctx (o, itr_src) (ktr_tgt tt) (ths, im_src, im_tgt1, st_src, st_tgt, r_shared)>>))
     :
     _geno tid geno RR f_src f_tgt r_ctx (o, itr_src) (trigger (Fair f) >>= ktr_tgt) (ths, im_src, im_tgt0, st_src, st_tgt, r_shared)
 
@@ -862,7 +163,7 @@ Section GENORDER.
       ths im_src im_tgt st_src st_tgt r_shared
       fn args ktr_src ktr_tgt
       (GENO: forall ret,
-             geno _ _ RR true true r_ctx (o, ktr_src ret) (ktr_tgt ret) (ths, im_src, im_tgt, st_src, st_tgt, r_shared))
+             geno RR true true r_ctx (o, ktr_src ret) (ktr_tgt ret) (ths, im_src, im_tgt, st_src, st_tgt, r_shared))
     :
     _geno tid geno RR f_src f_tgt r_ctx (o, trigger (Observe fn args) >>= ktr_src) (trigger (Observe fn args) >>= ktr_tgt) (ths, im_src, im_tgt, st_src, st_tgt, r_shared)
 
@@ -879,7 +180,7 @@ Section GENORDER.
                im_tgt2
                (TGT: fair_update im_tgt1 im_tgt2 (sum_fmap_l (tids_fmap tid ths1))),
         exists o1,
-          (<<GENO: geno _ _ RR f_src true r_ctx1 (o1, trigger (Yield) >>= ktr_src) (ktr_tgt tt) (ths1, im_src1, im_tgt2, st_src1, st_tgt1, r_shared1)>>) /\
+          (<<GENO: geno RR f_src true r_ctx1 (o1, trigger (Yield) >>= ktr_src) (ktr_tgt tt) (ths1, im_src1, im_tgt2, st_src1, st_tgt1, r_shared1)>>) /\
             (<<STUTTER: wf_stt.(lt) o1 o0>>))
     :
     _geno tid geno RR f_src f_tgt r_ctx0 (o0, trigger (Yield) >>= ktr_src) (trigger (Yield) >>= ktr_tgt) (ths0, im_src0, im_tgt0, st_src0, st_tgt0, r_shared0)
@@ -890,7 +191,7 @@ Section GENORDER.
       ktr_src itr_tgt
       (GENO: exists im_src1 o1,
           (<<FAIR: fair_update im_src0 im_src1 (sum_fmap_l (tids_fmap tid ths))>>) /\
-            (<<GENO: geno _ _ RR true f_tgt r_ctx (o1, ktr_src tt) itr_tgt (ths, im_src1, im_tgt, st_src, st_tgt, r_shared)>>))
+            (<<GENO: geno RR true f_tgt r_ctx (o1, ktr_src tt) itr_tgt (ths, im_src1, im_tgt, st_src, st_tgt, r_shared)>>))
     :
     _geno tid geno RR f_src f_tgt r_ctx (o0, trigger (Yield) >>= ktr_src) itr_tgt (ths, im_src0, im_tgt, st_src, st_tgt, r_shared)
 
@@ -906,9 +207,9 @@ Section GENORDER.
   Definition geno (tid: thread_id)
              R_src R_tgt (RR: R_src -> R_tgt -> URA.car -> shared_rel):
     bool -> bool -> URA.car -> (wf_stt.(T) * itree srcE R_src) -> itree tgtE R_tgt -> shared_rel :=
-    pind9 (_geno tid) top9 R_src R_tgt RR.
+    pind7 (@_geno tid R_src R_tgt) top7 RR.
 
-  Lemma geno_mon tid: monotone9 (_geno tid).
+  Lemma geno_mon tid R0 R1: monotone7 (@_geno tid R0 R1).
   Proof.
     ii. inv IN; try (econs; eauto; fail).
     { des. econs; eauto. }
@@ -932,72 +233,72 @@ Section GENORDER.
   Proof.
     remember (o0, src) as osrc.
     move GENO before tid. revert_until GENO.
-    pattern R0, R1, LRR, ps, pt, r_ctx, osrc, tgt, shr.
-    revert R0 R1 LRR ps pt r_ctx osrc tgt shr GENO. apply pind9_acc.
-    intros rr DEC IH. clear DEC. intros R0 R1 LRR ps pt r_ctx osrc tgt shr GENO.
+    pattern LRR, ps, pt, r_ctx, osrc, tgt, shr.
+    revert LRR ps pt r_ctx osrc tgt shr GENO. apply pind7_acc.
+    intros rr DEC IH. clear DEC. intros LRR ps pt r_ctx osrc tgt shr GENO.
     i; clarify.
-    eapply pind9_unfold in GENO; eauto with paco.
+    eapply pind7_unfold in GENO; eauto with paco.
     inv GENO.
 
-    { eapply pind9_fold. econs 1; eauto. }
-    { eapply pind9_fold. econs 2; eauto.
+    { eapply pind7_fold. econs 1; eauto. }
+    { eapply pind7_fold. econs 2; eauto.
       destruct GENO0 as [GENO IND]. eapply IH in IND; eauto. split; ss.
     }
-    { eapply pind9_fold. econs 3; eauto.
+    { eapply pind7_fold. econs 3; eauto.
       des. destruct GENO0 as [GENO IND]. eapply IH in IND; eauto. esplits; eauto.
       split; ss; eauto.
     }
-    { eapply pind9_fold. econs 4; eauto.
+    { eapply pind7_fold. econs 4; eauto.
       destruct GENO0 as [GENO IND]. eapply IH in IND; eauto. split; ss.
     }
-    { eapply pind9_fold. econs 5; eauto.
+    { eapply pind7_fold. econs 5; eauto.
       destruct GENO0 as [GENO IND]. eapply IH in IND; eauto. split; ss.
     }
-    { eapply pind9_fold. econs 6; eauto.
+    { eapply pind7_fold. econs 6; eauto.
       destruct GENO0 as [GENO IND]. eapply IH in IND; eauto. split; ss.
     }
-    { eapply pind9_fold. econs 7; eauto. }
-    { eapply pind9_fold. econs 8; eauto.
+    { eapply pind7_fold. econs 7; eauto. }
+    { eapply pind7_fold. econs 8; eauto.
       des. destruct GENO as [GENO IND]. eapply IH in IND; eauto. esplits; eauto.
       split; ss; eauto.
     }
 
-    { eapply pind9_fold. econs 9; eauto.
+    { eapply pind7_fold. econs 9; eauto.
       destruct GENO0 as [GENO IND]. eapply IH in IND; eauto. split; ss.
     }
-    { eapply pind9_fold. econs 10; eauto.
+    { eapply pind7_fold. econs 10; eauto.
       i. specialize (GENO0 x).
       destruct GENO0 as [GENO IND]. eapply IH in IND; eauto. split; ss.
     }
-    { eapply pind9_fold. econs 11; eauto.
+    { eapply pind7_fold. econs 11; eauto.
       destruct GENO0 as [GENO IND]. eapply IH in IND; eauto. split; ss.
     }
-    { eapply pind9_fold. econs 12; eauto.
+    { eapply pind7_fold. econs 12; eauto.
       destruct GENO0 as [GENO IND]. eapply IH in IND; eauto. split; ss.
     }
-    { eapply pind9_fold. econs 13; eauto.
+    { eapply pind7_fold. econs 13; eauto.
       destruct GENO0 as [GENO IND]. eapply IH in IND; eauto. split; ss.
     }
-    { eapply pind9_fold. econs 14; eauto.
+    { eapply pind7_fold. econs 14; eauto.
       i. specialize (GENO0 _ FAIR).
       destruct GENO0 as [GENO IND]. eapply IH in IND; eauto. split; ss.
     }
-    { eapply pind9_fold. econs 15; eauto.
+    { eapply pind7_fold. econs 15; eauto.
       i. specialize (GENO0 ret).
       destruct GENO0 as [GENO IND]. eapply IH in IND; eauto. split; ss.
     }
 
-    { eapply pind9_fold. econs 16; eauto.
+    { eapply pind7_fold. econs 16; eauto.
       i. specialize (GENO0 _ _ _ _ _ _ _ INV0 VALID0 _ TGT). des. esplits; eauto.
       destruct GENO as [GENO IND]. eapply IH in IND; eauto. split; ss.
     }
 
-    { eapply pind9_fold. econs 17; eauto.
+    { eapply pind7_fold. econs 17; eauto.
       des. esplits; eauto.
-      eapply upind9_mon; eauto. ss.
+      eapply upind7_mon; eauto. ss.
     }
 
-    { eapply pind9_fold. econs 18; eauto. }
+    { eapply pind7_fold. econs 18; eauto. }
 
   Qed.
 
@@ -1016,32 +317,32 @@ Section GENORDER.
     set (fzero:= fun _: (A R0 R1) => @ord_tree_base (A R0 R1)). set (one:= ord_tree_cons fzero).
     inv LSIM.
 
-    { exists one. eapply pind9_fold. econs 1; eauto.
+    { exists one. eapply pind7_fold. econs 1; eauto.
       instantiate (1:=fzero (ps, pt, r_ctx, Ret r_src, Ret r_tgt, (ths, im_src, im_tgt, st_src, st_tgt, r_shared))); ss.
     }
 
     { destruct LSIM0 as [LSIM IND]. eapply IH in IND. des.
-      exists o. eapply pind9_fold. econs 2; eauto. split; ss.
+      exists o. eapply pind7_fold. econs 2; eauto. split; ss.
     }
     { des. destruct LSIM0 as [LSIM IND]. eapply IH in IND. des.
-      exists o. eapply pind9_fold. econs 3; eauto. eexists. split; ss. eauto.
+      exists o. eapply pind7_fold. econs 3; eauto. eexists. split; ss. eauto.
     }
     { destruct LSIM0 as [LSIM IND]. eapply IH in IND. des.
-      exists o. eapply pind9_fold. econs 4; eauto. split; ss.
+      exists o. eapply pind7_fold. econs 4; eauto. split; ss.
     }
     { destruct LSIM0 as [LSIM IND]. eapply IH in IND. des.
-      exists o. eapply pind9_fold. econs 5; auto. split; ss.
+      exists o. eapply pind7_fold. econs 5; auto. split; ss.
     }
     { destruct LSIM0 as [LSIM IND]. eapply IH in IND. des.
-      exists o. eapply pind9_fold. econs 6; auto. split; ss.
+      exists o. eapply pind7_fold. econs 6; auto. split; ss.
     }
-    { exists one. eapply pind9_fold. econs 7; eauto. }
+    { exists one. eapply pind7_fold. econs 7; eauto. }
     { des. destruct LSIM as [LSIM IND]. eapply IH in IND. des.
-      exists o. eapply pind9_fold. econs 8; eauto. esplits; eauto. split; ss.
+      exists o. eapply pind7_fold. econs 8; eauto. esplits; eauto. split; ss.
     }
 
     { destruct LSIM0 as [LSIM IND]. eapply IH in IND. des. exists o.
-      eapply pind9_fold. econs 9; eauto. ss.
+      eapply pind7_fold. econs 9; eauto. ss.
     }
 
     { hexploit ord_tree_join.
@@ -1053,7 +354,7 @@ Section GENORDER.
         eauto.
       }
       intro JOIN. des. exists o1.
-      eapply pind9_fold. econs 10.
+      eapply pind7_fold. econs 10.
       i. specialize (LSIM0 x). destruct LSIM0 as [LSIM IND].
       specialize (JOIN (ps, true, r_ctx, src, (ktr_tgt x), (ths, im_src, im_tgt, st_src, st_tgt, r_shared))).
       destruct JOIN; auto. des. split; ss.
@@ -1061,13 +362,13 @@ Section GENORDER.
     }
 
     { destruct LSIM0 as [LSIM IND]. eapply IH in IND. des. exists o.
-      eapply pind9_fold. econs 11; eauto. ss.
+      eapply pind7_fold. econs 11; eauto. ss.
     }
     { destruct LSIM0 as [LSIM IND]. eapply IH in IND. des. exists o.
-      eapply pind9_fold. econs 12; eauto. ss.
+      eapply pind7_fold. econs 12; eauto. ss.
     }
     { destruct LSIM0 as [LSIM IND]. eapply IH in IND. des. exists o.
-      eapply pind9_fold. econs 13; eauto. ss.
+      eapply pind7_fold. econs 13; eauto. ss.
     }
 
     { hexploit ord_tree_join.
@@ -1079,7 +380,7 @@ Section GENORDER.
         eauto.
       }
       intro JOIN. des. exists o1.
-      eapply pind9_fold. econs 14.
+      eapply pind7_fold. econs 14.
       i. specialize (LSIM0 _ FAIR). destruct LSIM0 as [LSIM IND].
       specialize (JOIN (ps, true, r_ctx, src, (ktr_tgt ()), (ths, im_src, im_tgt1, st_src, st_tgt, r_shared))).
       destruct JOIN; auto. des. split; ss.
@@ -1095,7 +396,7 @@ Section GENORDER.
         eauto.
       }
       intro JOIN. des. exists o1.
-      eapply pind9_fold. econs 15.
+      eapply pind7_fold. econs 15.
       i. specialize (LSIM0 ret). destruct LSIM0 as [LSIM IND].
       specialize (JOIN (true, true, r_ctx, ktr_src ret, ktr_tgt ret, (ths, im_src, im_tgt, st_src, st_tgt, r_shared))).
       destruct JOIN; auto. des. split; ss.
@@ -1111,7 +412,7 @@ Section GENORDER.
         eauto.
       }
       intro JOIN. des. exists o1.
-      eapply pind9_fold. econs 16.
+      eapply pind7_fold. econs 16.
       1,2: eauto.
       i. specialize (LSIM0 _ _ _ _ _ _ _ INV0 VALID0 _ TGT). destruct LSIM0 as [LSIM IND].
       specialize (JOIN (ps, true, r_ctx1, (x <- trigger Yield;; ktr_src x), ktr_tgt (), (ths1, im_src1, im_tgt2, st_src1, st_tgt1, r_shared1))).
@@ -1119,11 +420,11 @@ Section GENORDER.
     }
 
     { des. destruct LSIM as [LSIM IND]. eapply IH in IND. des. exists o.
-      eapply pind9_fold. econs 17; eauto. esplits; eauto.
+      eapply pind7_fold. econs 17; eauto. esplits; eauto.
       split; ss. eauto.
     }
 
-    { exists one. eapply pind9_fold. econs 18. pclearbot. auto. }
+    { exists one. eapply pind7_fold. econs 18. pclearbot. auto. }
 
   Qed.
 
@@ -1162,94 +463,6 @@ Section PROOF.
 
   Variable I: shared_rel.
 
-  Lemma stutter_ord_weak
-          wf_stt tid
-          R0 R1 (LRR: R0 -> R1 -> URA.car -> shared_rel)
-          ps pt r_ctx src tgt (shr: shared) o0 o1
-          (LE: wf_stt.(le) o0 o1)
-          (LSIM: ModSimStutter.lsim wf_stt I tid LRR ps pt r_ctx (o0, src) tgt shr)
-    :
-    ModSimStutter.lsim wf_stt I tid LRR ps pt r_ctx (o1, src) tgt shr.
-  Proof.
-    destruct LE as [EQ | LT].
-    { clarify. }
-    revert_until tid. pcofix CIH; i.
-    remember (o0, src) as osrc.
-    move LSIM before CIH. revert_until LSIM.
-    punfold LSIM.
-    pattern R0, R1, LRR, ps, pt, r_ctx, osrc, tgt, shr.
-    revert R0 R1 LRR ps pt r_ctx osrc tgt shr LSIM. apply pind9_acc.
-    intros rr DEC IH. clear DEC. intros R0 R1 LRR ps pt r_ctx osrc tgt shr LSIM.
-    i; clarify.
-    eapply pind9_unfold in LSIM.
-    2:{ eapply ModSimStutter._lsim_mon. }
-    inv LSIM.
-
-    { pfold. eapply pind9_fold. econs 1; eauto. }
-    { pfold. eapply pind9_fold. econs 2; eauto.
-      split; ss. destruct LSIM0 as [LSIM IND]. eapply IH in IND; eauto. punfold IND.
-    }
-    { pfold. eapply pind9_fold. econs 3; eauto.
-      des. exists x.
-      split; ss. destruct LSIM0 as [LSIM IND]. eapply IH in IND; eauto. punfold IND.
-    }
-    { pfold. eapply pind9_fold. econs 4; eauto.
-      split; ss. destruct LSIM0 as [LSIM IND]. eapply IH in IND; eauto. punfold IND.
-    }
-    { pfold. eapply pind9_fold. econs 5; eauto.
-      split; ss. destruct LSIM0 as [LSIM IND]. eapply IH in IND; eauto. punfold IND.
-    }
-    { pfold. eapply pind9_fold. econs 6; eauto.
-      split; ss. destruct LSIM0 as [LSIM IND]. eapply IH in IND; eauto. punfold IND.
-    }
-    { pfold. eapply pind9_fold. econs 7; eauto. }
-    { pfold. eapply pind9_fold. econs 8; eauto.
-      des. esplits; eauto.
-      split; ss. destruct LSIM as [LSIM IND]. eapply IH in IND; eauto. punfold IND.
-    }
-    { pfold. eapply pind9_fold. econs 9; eauto.
-      split; ss. destruct LSIM0 as [LSIM IND]. eapply IH in IND; eauto. punfold IND.
-    }
-    { pfold. eapply pind9_fold. econs 10; eauto.
-      i. specialize (LSIM0 x).
-      split; ss. destruct LSIM0 as [LSIM IND]. eapply IH in IND; eauto. punfold IND.
-    }
-    { pfold. eapply pind9_fold. econs 11; eauto.
-      split; ss. destruct LSIM0 as [LSIM IND]. eapply IH in IND; eauto. punfold IND.
-    }
-    { pfold. eapply pind9_fold. econs 12; eauto.
-      split; ss. destruct LSIM0 as [LSIM IND]. eapply IH in IND; eauto. punfold IND.
-    }
-    { pfold. eapply pind9_fold. econs 13; eauto.
-      split; ss. destruct LSIM0 as [LSIM IND]. eapply IH in IND; eauto. punfold IND.
-    }
-    { pfold. eapply pind9_fold. econs 14; eauto.
-      i. specialize (LSIM0 _ FAIR).
-      split; ss. destruct LSIM0 as [LSIM IND]. eapply IH in IND; eauto. punfold IND.
-    }
-    { pfold. eapply pind9_fold. econs 15; eauto.
-      i. specialize (LSIM0 ret). pclearbot.
-      right. eapply CIH; eauto.
-    }
-
-    { pfold. eapply pind9_fold. eapply ModSimStutter.lsim_yieldR; eauto.
-      i. hexploit LSIM0; clear LSIM0; eauto; intro LSIM. des. esplits; eauto.
-      pclearbot. right. eapply CIH; eauto.
-    }
-
-    { pfold. eapply pind9_fold. eapply ModSimStutter.lsim_yieldL; eauto.
-      des. esplits; eauto. destruct LSIM as [LSIM IND].
-      split; ss. eapply pind9_mon_gen. eapply LSIM.
-      - i. eapply __lsim_mon. 2: eapply PR. i. eapply upaco9_mon_bot; eauto.
-      - ss.
-    }
-
-    { pfold. eapply pind9_fold. eapply ModSimStutter.lsim_progress.
-      pclearbot. right. eapply CIH; eauto.
-    }
-
-  Qed.
-
   Definition lift_wf (wf: WF): WF := sum_WF (sum_WF wf wf) wf.
 
   Definition mk_o (wf: WF) (w: wf.(T)) R (o: wf.(T)) (ps: bool) (itr_src: itree srcE R):
@@ -1280,46 +493,25 @@ Section PROOF.
   Proof.
     eapply nosync_geno in LSIM. des.
     exists (mk_o (@wf_ot R0 R1) (@ord_tree_base _) o ps src).
-    revert_until R1. ginit. gcofix CIH; i.
+    revert_until R1. pcofix CIH; i.
     remember (o, src) as osrc.
-    remember R0 as _R0. remember R1 as _R1.
-    move R0 after CIH. move R1 after CIH. move CIH before tid.
-    remember src as _src. remember tgt as _tgt. remember o as _o.
-    assert (__src: itree srcE R0).
-    { rewrite <- Heq_R0. exact src. }
-    assert (Heq_src_: __src = src).
-
-    rewrite Heq_R0 in src.
-    setoid_rewrite HeqR_src in src.
-    revert_until HeqR_src. rewrite !HeqR_tgt.
-    pattern R_src, R_tgt, LRR, ps, pt, r_ctx, osrc, tgt, shr.
     move LSIM before CIH. revert_until LSIM.
-    pattern R_src, R_tgt, LRR, ps, pt, r_ctx, osrc, tgt, shr.
-    revert R0 R1 LRR ps pt r_ctx osrc tgt shr LSIM. apply pind9_acc.
-    intros rr DEC IH. clear DEC. intros R0 R1 LRR ps pt r_ctx osrc tgt shr LSIM.
+    pattern LRR, ps, pt, r_ctx, osrc, tgt, shr.
+    revert LRR ps pt r_ctx osrc tgt shr LSIM. apply pind7_acc.
+    intros rr DEC IH. clear DEC. intros LRR ps pt r_ctx osrc tgt shr LSIM.
     intros src o Eosrc. clarify.
-    eapply pind9_unfold in LSIM; eauto with paco.
+    eapply pind7_unfold in LSIM; eauto with paco.
     inv LSIM.
 
-    remember (o, src) as osrc. ss.
-    move LSIM before tid. revert_until LSIM.
-    pattern R0, R1, LRR, ps, pt, r_ctx, osrc, tgt, shr.
-    revert R0 R1 LRR ps pt r_ctx osrc tgt shr LSIM. apply pind9_acc.
-    intros rr DEC IH. clear DEC. intros R0 R1 LRR ps pt r_ctx osrc tgt shr LSIM.
-    intros src o Eosrc. clarify.
-    eapply pind9_unfold in LSIM; eauto with paco.
-    inv LSIM.
-
-    { unfold mk_o. des_ifs.
-      - pfold. eapply pind9_fold. econs 1; eauto.
-        instantiate (1:=inl (inl o1)). ss. econs 3.
-      - pfold. eapply pind9_fold. econs 1; eauto.
-        instantiate (1:=inl (inl o1)). ss. econs 3.
+    { pfold. eapply pind9_fold. econs 1; eauto.
+      instantiate (1:=inl (inl o1)). ss.
+      unfold mk_o. des_ifs. all: econs 3.
     }
 
     { destruct GENO as [GENO IND]. eapply IH in IND; eauto.
       pfold. eapply pind9_fold. econs 2; eauto.
       split; ss.
+      
       eapply stutter_ord_weak in IND. punfold IND.
       unfold mk_o. des_ifs; try reflexivity.
       - right. ss. econs 3.
